\documentclass[12pt]{article}
\usepackage{bbm}
\usepackage{amsmath}
\usepackage{amsthm}
\usepackage{amssymb}
\usepackage{mathtools}
\DeclarePairedDelimiter\ceil{\lceil}{\rceil}
\DeclarePairedDelimiter\floor{\lfloor}{\rfloor}
\begin{document}

define $O(x,y,z,\bar{x},\bar{y},\bar{z},w,\bar{w},MP,SP,H,R) = (a,b,c,d,e,f,MP_l,SP_l)$.

\begin{align*}
e &= \mathbbm{1}\{5 \leq R <20\}	+2* \mathbbm{1}\{20 \leq R <40\} +	3*\mathbbm{1}\{40 \leq R <60\}\\
&+ 4*\mathbbm{1}\{60 \leq R <80\}	+ 5*\mathbbm{1}\{R \leq 100\} 
\end{align*}

Here $\floor*{5.4} = 5$ means round down.
\begin{align*}
	f = 0 \quad &\text{if $MP \geq g((x+0.25z)w,yw,w) - 5.5w + g(x+0.25z,y,w)+4 + \floor*{\frac{R}{10}}$}\quad \\ &\text{and if $MP \geq g((\bar{x}+0.25\bar{z})\bar{w},\bar{y}\bar{w},\bar{w}) - 5.5\bar{w} + g(\bar{x}+0.25\bar{z},\bar{y},\bar{w})+4 + \floor*{\frac{R}{10}}$}\\ &\text{otherwise,}
\end{align*}

\begin{equation*}
  f =
    \begin{cases}
      1 & \frac{g(x+0.25z,y,w)-5.5w}{g((x+0.25z)w,yw,w) - 5.5w + g(x+0.25z,y,w)} \geq \frac{g(\bar{x}+0.25\bar{z},\bar{y},\bar{w})-5.5\bar{w}}{g((\bar{x}+0.25\bar{z})\bar{w},\bar{y}\bar{w},\bar{w}) - 5.5\bar{w} + g(\bar{x}+0.25\bar{z},\bar{y},\bar{w})}  \\
      2 & \frac{g(x+0.25z,y,w)-5.5w}{g((x+0.25z)w,yw,w) - 5.5w + g(x+0.25z,y,w)} < \frac{g(\bar{x}+0.25\bar{z},\bar{y},\bar{w})-5.5\bar{w}}{g((\bar{x}+0.25\bar{z})\bar{w},\bar{y}\bar{w},\bar{w}) - 5.5\bar{w} + g(\bar{x}+0.25\bar{z},\bar{y},\bar{w})}  \\
    \end{cases}       
\end{equation*}
\begin{align*}
& c = 2 \quad \text{if $f = 1$ or $f=2$ }\\
&c=0 \quad\text{otherwise}	
\end{align*}
 \begin{align*}
& d = \floor*{\frac{MP-e}{4}} \quad \text{if $f = 0$ for previous $4$ sequential turns }\\
&d=0 \quad\text{otherwise}	
\end{align*}
\begin{align*}
& a = g((\bar{x}+0.25\bar{z})\bar{w},\bar{y}\bar{w},\bar{w}) \quad \text{if $f = 1$}\\
& a = g((x+0.25z)w,yw,w) \quad \text{if $ f = 2$ }\\
&a=0 \quad\text{if f = 0}	
\end{align*}
 \begin{align*}
& b = MP-a \quad \text{if $f = 1$ or $f = 2$}\\
&b=0 \quad\text{if f = 0}	
\end{align*}

$g$ is defined below:
\begin{equation*}
g(i,j,t) =5.5t +2i+3j  	
\end{equation*}

\begin{equation*}
SP_l = SP - c	
\end{equation*}

\begin{equation*}
SP_l = SP - a -b - 2d -e	
\end{equation*}
\end{document}
